Flapjack/Test/Backend.lean
@@ -13,6 +13,8 @@ import Flapjack.Test.MustTerminate
 import Flapjack.Test.TailCalls
 import Flapjack.Test.WordOperations
 import Flapjack.Test.WordBitmaps
+import Flapjack.Test.BitmapPipeline
+import Flapjack.Test.HeapAlloc
 import Flapjack.Test.WordToStack
 import Flapjack.Test.ParallelMove
 import Flapjack.Test.Stack
